normalize

lib/bv32_ops.dfy
@@ -156,4 +156,20 @@ module bv32_ops refines generic_bv_ops
     {
         sub(x, y)
     }
+
+    function method uint32_rsai(x: uint, amount: uint): uint
+        requires amount < 32;
+    {
+        to_uint32(int32_rs(to_int32(x), amount))
+    }
+
+    function method uint32_lh(x: uint): integers.uint16
+    {
+        lh(x)
+    }
+
+    function method uint32_uh(x: uint): integers.uint16
+    {
+        uh(x)
+    }
 }
